update notes from 3/16 class

Notes4/IndPred.lean
@@ -1,9 +1,13 @@
+import Mathlib.Data.Nat.Basic
+
 /- 
 # Sorting a list
 
 -/
 
-variable {α : Type} {f : α → α → Bool} (r : α → α → Prop) 
+namespace Notes
+
+variable {α : Type} (f : α → α → Bool) (r : α → α → Prop) 
 
 /- 
 We sort lists of type `α` using the comparison function 
@@ -32,6 +36,7 @@ inductive Sorted (f : α → α → Bool) : List α → Prop where
 
 open Sorted
 
+/- We can check that particular lists are `Sorted` -/
 example : Sorted (·≤·) [1,2,3] := by 
   apply longer
   · simp 
@@ -39,12 +44,26 @@ example : Sorted (·≤·) [1,2,3] := by
     · simp 
     · apply single
 
+/- We can also prove basic facts about our implementation 
+of sorted lists -/
 theorem sorted_tail_of_sorted (a : α) (as : List α) 
     (h : Sorted f (a::as)) : Sorted f as := by
   match h with 
   | single => apply nil  
   | longer _ h'' => exact h''
 
+/- We now we want to implement an algortihm to sort 
+lists and then _prove_ that it always produces a `Sorted` 
+list. 
+
+We will use insert sort. We will recursively sort the 
+tail of a list and then insert the head in the 
+appropriate place. We first give the insertion function.-/
+
+/-- 
+`insert` places `a` before the first element `a'` 
+of `l` which satisfies `f a a'`. 
+-/
 def insert (a : α) (l : List α) : List α :=
   match l with 
   | [] => [a] 
@@ -55,4 +74,97 @@ def insert (a : α) (l : List α) : List α :=
 
 #check insert 
 
-def insertSort (l : List α) : List α := sorry 
+/- We prove a basic result about the length of inserted 
+list and tag it with `@[simp]` for use with `simp` -/
+@[simp]
+theorem len_insert_eq_succ_len {a : α} {l : List α} : 
+    (insert f a l).length = l.length + 1 := by 
+  match l with 
+  | [] => simp [insert]
+  | a'::as =>
+    match h : f a a' with 
+    | true => simp [insert, h]
+    | false => simp [insert, h]; apply len_insert_eq_succ_len 
+
+/--
+We sort `l` recursively sorting the tail first and then 
+inserting the head at the appropriate location.
+-/
+def insertSort (l : List α) : List α :=
+  match l with 
+  | [] => [] 
+  | a::as => insert f a <| insertSort as
+
+#check insertSort
+
+/- Some examples our polymorphic sorting algorithm applies to -/
+#eval insertSort (·≤·) [4,5,2,4,5,6]
+#eval insertSort (fun (b b' : Bool) => b && b') [true,false,false]
+#eval insertSort (fun _ _ => true) [4,5,2,4,5,6]
+
+
+/- For a general `f`, we will not be able to show that the 
+output of `insert f l` satsisfies `Sorted f l`. For example, 
+for `fun _ _ => false`, if we have `Sorted f l` then 
+`l.length` is 0 or 1. This is a reasonable class of `f` to 
+make sorting work as expected -/
+class Asymmetric (f : α → α → Bool) where
+  asym {a a'} : !f a a' → f a' a
+
+open Asymmetric
+
+/- A helpful constructor for `Sorted` that unifies the 
+nonempty cases -/
+def Sorted.cons {a : α} {l : List α} (h₁ : Sorted f l) 
+    (h₂ : l.length > 0) (h₃ : f a l[0]) : Sorted f (a::l) :=
+  match h₁ with 
+  | nil => single
+  | single => longer h₃ single
+  | longer h h' => longer h₃ <| longer h h'
+
+/- If we have a `Sorted` list with at least two elements, 
+then the first elements are ordered appropriately with 
+respect to `f` -/
+theorem ordered_of_sorted {a a' : α} {as : List α} 
+    (h : Sorted f (a::a'::as)) : f a a' :=
+  match h with 
+  | longer h' _ => h'
+
+/- If we have a `Sorted` list `a'::as` where `a` and `a'` are 
+ordered wrong, then the first two elements of `a'::insert f a as` 
+are ordered correctly -/
+theorem ordered_cons_insert_of_unordered {a a' : α} {as : List α}
+    (h : Sorted f (a'::as)) (h' : f a' a) : f a' (insert f a as)[0] :=
+  match as with 
+  | [] => by simpa [insert]
+  | a''::as' => 
+  match h'' : f a a'' with 
+    | true => by simpa [insert, h'']
+    | false => by simp [insert, h'']; apply ordered_of_sorted f h
+
+/- We prove that if we insert an element into a `Sorted` list 
+it will remain `Sorted` assuming `f` is `Asymmetric` -/
+theorem insert_sorted_of_sorted {a : α} {l : List α} [Asymmetric f] 
+    (h : Sorted f l) : Sorted f <| insert f a l :=
+  match l with 
+  | [] => single
+  | a'::as =>
+    match h' : f a a' with 
+    | true => by simp [insert, h']; apply longer h' h 
+    | false => by
+      simp [insert, h']
+      apply cons f
+      · apply insert_sorted_of_sorted <| sorted_tail_of_sorted f a' as h   
+      · apply ordered_cons_insert_of_unordered f h 
+        · apply asym; simp; assumption
+
+/- Finally, we prove that if `f` is `Asymmetric` then `insertSort` 
+always produces a `Sorted` list no matter `α` or `f` -/
+theorem sorted_of_insertSort (l : List α) [Asymmetric f] : 
+    Sorted f <| insertSort f l :=
+  match l with 
+  | [] => nil
+  | a::as => by
+    dsimp [insertSort]
+    apply insert_sorted_of_sorted f <| sorted_of_insertSort as
+
